iso_dh/shared.v
@@ -84,7 +84,6 @@ Definition msg2_pred kR m2 : iProp :=
     let gb := TExp (TInt 0) b in
     let gab := TExp ga b in
     let secret := Spec.of_list [ga; gb; gab] in
-    let kS := Spec.tag (nroot.@"keys".@"sym") secret in
     ⌜m2 = Spec.of_list [ga; gb; vkI]⌝ ∗
     minted_at n ga ∗
     (public b ↔ ▷ □ ((∃ kI, ⌜vkI = TKey Dec kI⌝ ∗ public_at n (TKey Enc kI)) ∨
@@ -92,21 +91,20 @@ Definition msg2_pred kR m2 : iProp :=
     (∀ t, dh_pred b t ↔ ▷ □ iso_dh_pred t) ∗
     escrow cryptisN
       (term_token ga ⊤)
-      (term_token kS (↑nroot.@"client")) ∗
-    term_meta kS (nroot.@"info") (vkI, TKey Dec kR, n).
+      (term_token secret (↑nroot.@"client")) ∗
+    term_meta secret (nroot.@"info") (vkI, TKey Dec kR, n).
 
 Definition msg3_pred kI m3 : iProp :=
   ∃ a gb kR n,
     let ga := TExp (TInt 0) a in
     let gab := TExp gb a in
     let secret := Spec.of_list [ga; gb; gab] in
-    let kS := Spec.tag (nroot.@"keys".@"sym") secret in
     ⌜m3 = Spec.of_list [ga; gb; TKey Dec kR]⌝ ∗
     (public a ↔ ▷ □ (public_at n (TKey Enc kI) ∨
                      public_at n (TKey Enc kR))) ∗
     (∀ t, dh_pred a t ↔ ▷ □ iso_dh_pred t) ∗
     (public_at n (TKey Enc kR) ∨
-     term_meta kS (nroot.@"info") (TKey Dec kI, TKey Dec kR, n)).
+     term_meta secret (nroot.@"info") (TKey Dec kI, TKey Dec kR, n)).
 
 Definition iso_dh_ctx : iProp :=
   enc_pred (N.@"m2") msg2_pred ∗
