store/connection_proofs.v
@@ -53,7 +53,15 @@ wp_alloc ts as "ts". set  si := SessInfo _ _ _ _. wp_pures.
 iDestruct "resP" as "(#m_kS & #p_kS & sess)".
 iRight. iModIntro. iExists _.  iSplit => //.
 iApply ("post" $! (ConnState si ts Init)). iFrame => /=.
-do !iSplit => //; iDestruct "sess" as "[fail|[sess token]]"; eauto.
+do !iSplit => //.
+- iDestruct "sess" as "[fail|[sess token]]"; eauto.
+- iIntros "!> %kt". iSplit.
+  + iIntros "#p_k".
+    iPoseProof (public_sym_keyE with "[//] p_k") as ">?".
+    by iApply "p_kS".
+  + iIntros "#fail". iApply public_sym_key => //.
+    iSplit => //. iModIntro. by iApply "p_kS".
+- iDestruct "sess" as "[fail|[sess token]]"; eauto.
 Qed.
 
 Lemma wp_connection_listen N c kR dq n :
@@ -84,7 +92,13 @@ iDestruct "resP" as "(%kI & -> & #p_vkI & #m_kS & #p_kS & #sess & token)".
 set  si := SessInfo _ _ _ _. wp_pures.
 iRight. iModIntro. iExists _.  iSplit => //.
 iApply ("post" $! (ConnState si ts Resp)). iFrame => /=.
-eauto 10.
+do !iSplit => //; eauto.
+iIntros "!> %kt". iSplit.
+- iIntros "#p_k".
+  iPoseProof (public_sym_keyE with "[//] p_k") as ">?".
+  by iApply "p_kS".
+- iIntros "#fail". iApply public_sym_key => //.
+  iSplit => //. iModIntro. by iApply "p_kS".
 Qed.
 
 Lemma wp_connection_timestamp cs (n : nat) :
@@ -116,7 +130,8 @@ Lemma wp_connection_session_key cs n :
       is_conn_state cs n ∗
       (session_fail cs ∨ session cs) ∗
       minted (si_key cs) ∗
-      □ (∀ kt, public (TKey kt (si_key cs)) ↔ ▷ session_fail cs) }}}.
+      □ (∀ kt, public (TKey kt (Spec.tag (nroot.@"keys".@"sym") (si_key cs)))
+                 ↔ ▷ session_fail cs) }}}.
 Proof.
 rewrite /Connection.session_key.
 iIntros "%Φ (? & #? & #? & #?) post". wp_pures. iApply "post".
@@ -148,7 +163,7 @@ iApply wp_send => //.
     - iApply "sec". by eauto.
     - by rewrite public_tag. }
   iApply public_TEncIS => //.
-  - by rewrite minted_TKey.
+  - by rewrite minted_TKey minted_tag.
   - iModIntro. iExists cs. by do !iSplit => //.
   - by iApply public_minted.
   - by iIntros "!> !> _". }
@@ -226,7 +241,8 @@ Qed.
 Lemma wp_connection_make_handlers φ Φ k (handlers : list (namespace * expr)) :
   ([∗ list] handler ∈ handlers,
       WP (handler.2 : expr) {{ f, □ ∀ m : term,
-        public (TEnc (TKey Enc k) (Spec.tag handler.1 m)) -∗
+        public (TEnc (TKey Enc (Spec.tag (nroot.@"keys".@"sym") k))
+                  (Spec.tag handler.1 m)) -∗
         φ -∗
         WP (f : val) m {{ v,
             ⌜v = NONEV⌝ ∗ φ ∨
@@ -234,7 +250,7 @@ Lemma wp_connection_make_handlers φ Φ k (handlers : list (namespace * expr)) :
   WP Connection.make_handlers handlers {{ v',
     ∃ handlers' : list val, ⌜v' = repr handlers'⌝ ∗
       [∗ list] handler' ∈ handlers', □ ∀ m : term,
-        public (TEnc (TKey Enc k) m) -∗
+        public (TEnc (TKey Enc (Spec.tag (nroot.@"keys".@"sym") k)) m) -∗
         φ -∗
         WP (handler' : val) m {{ v,
           ⌜v = NONEV⌝ ∗ φ ∨
@@ -303,6 +319,7 @@ iApply (wp_wand with "[wps]").
       iDestruct "p_m" as "(%si & %e_kS & #sess' & p_m & inv_m)".
       iSplit => //.
       iDestruct "sess" as "[fail|sess]"; first by eauto.
+      case/Spec.tag_inj: e_kS => _ e_kS.
       iPoseProof (session_agree with "sess' sess") as "->" => //.
       by eauto. }
   iApply ("wp" with "p_m [//] conn inv"). }
@@ -359,6 +376,7 @@ iAssert (▷ □ (public m ∗ (session_fail cs ∨ Φ cs m)))%I
     iDestruct "p_m" as "(%si & %e_kS & #sess' & p_m & inv_m)".
     iSplit => //.
     iDestruct "sess" as "[fail|sess]"; first by eauto.
+    case/Spec.tag_inj: e_kS => _ e_kS.
     iPoseProof (session_agree with "sess' sess") as "->" => //.
     by eauto. }
 iMod (lc_fupd_elim_later with "c p_m") as "{p_m} [#p_m #inv_m]".
