tactics.v
@@ -156,7 +156,7 @@ by rewrite envs_entails_unseal => H; rewrite -wp_bind -wp_tsenc.
 Qed.
 
 Lemma tac_wp_tsdec Γ E K c k t Ψ :
-  (∀ t', t = TEnc (TKey Enc k) (Spec.tag c t') →
+  (∀ t', t = TEnc (TKey Enc (Spec.tag (nroot.@"keys".@"sym") k)) (Spec.tag c t') →
          envs_entails Γ (WP fill K (Val (SOMEV t')) @ E {{ Ψ }})) →
   (Spec.tsdec c (Spec.mkskey k) t = None →
    envs_entails Γ (WP fill K (Val NONEV) @ E {{ Ψ }})) →
